Main.lean
@@ -7,13 +7,11 @@ def myPrometheusEnv : Environment := {
   scrapeConfigs := [{ targetLabels := ["job", "instance"], exporter := node_exporter }]
 }
 
-def myDashboard : Dashboard node_exporter := { name := "My Dashboard", panels := [
+def myDashboard : Dashboard myPrometheusEnv := { name := "My Dashboard", panels := [
     (Panel.graph { promql := { v := [pql| node_filesystem_avail_bytes{fstype="f"} ] } }),
-    (Panel.graph { promql := { v := [pql| process_cpu_seconds_total] } }),
+    (Panel.graph { promql := { v := [pql| process_cpu_seconds_total{job="linux"} ]}}),
     (Panel.graph { promql := { v := [pql| rate(node_network_receive_bytes_total{device="eth0"}[120])] } })
-  ] }
-
-#check @Panel.graph node_exporter { promql := { v := [pql| rate(node_network_receive_bytes_total{device="eth0"}[120]) ] } }
+]}
 
 def main : IO Unit := do
   IO.print $ Lean.toJson $ dashboardToGrafana myDashboard
